steel/Zeta.Steel.LogEntry.fsti
@@ -29,7 +29,7 @@ inline_for_extraction
 noextract
 let parser_u256 : parser spec_parser_u256 = zeta__parser_u256
 
-val zeta__serialize_timestamp : serializer spec_serialize_timestamp
+val zeta__serialize_timestamp : serializer spec_serializer_timestamp
 
 noextract
 let timestamp_len = 8
@@ -42,17 +42,27 @@ let seq_suffix_is_zero (s:Seq.seq byte)
 
 module A = Steel.ST.Array
 open Steel.ST.Util
+open Zeta.Steel.Util
+
 let serialize_timestamp (#bs:Ghost.erased (Seq.seq FStar.UInt8.t))
                         (a:byte_array { A.length a == 8 })
                         (v: timestamp)
  : STT U32.t
     (A.pts_to a full_perm bs)
     (fun slice_len ->
-       exists_ (fun (bs:_) ->
+       exists_ (fun (bs:bytes) ->
          A.pts_to a full_perm bs `star`
          pure (
-           spec_serialize_timestamp v == bs)))
- = admit_(); return 0ul
+           spec_serializer_timestamp v == bs)))
+ = intro_exists_erased bs (array_pts_to a);
+   let n = zeta__serialize_timestamp 8ul 0ul a v in
+   let bs = elim_exists () in
+   elim_pure _;
+   // intro_pure (eq2 #bytes (spec_serializer_timestamp v) bs);
+   // intro_exists_erased bs (fun (bs:bytes) -> A.pts_to a full_perm bs `star`
+   //                                        pure (spec_serializer_timestamp v == bs));
+   return n
+   
 
 let seq_suffix_is_zero_elim (s:Seq.seq byte)
                             (from:nat)
@@ -63,7 +73,7 @@ let seq_suffix_is_zero_elim (s:Seq.seq byte)
          Seq.slice s from (Seq.length s) `Seq.equal` Seq.create (Seq.length s - from) 0uy)
   = ()
 
-
+#push-options "--z3rlimit_factor 3 --fuel 0 --ifuel 0 --query_stats"
 let serialize_iv (a:byte_array { A.length a == 96 })
                  (v: timestamp)
   : Steel.ST.Util.STT unit
@@ -73,7 +83,7 @@ let serialize_iv (a:byte_array { A.length a == 96 })
          A.pts_to a full_perm bs `star`
          pure (
            seq_suffix_is_zero bs timestamp_len /\
-           spec_serialize_iv v == bs)))
+           spec_serializer_iv v == bs)))
   = let bs = elim_exists () in
     A.pts_to_length a bs;
     elim_pure _;
@@ -87,7 +97,8 @@ let serialize_iv (a:byte_array { A.length a == 96 })
              A.pts_to (A.split_r a 8sz) full_perm (Seq.slice bs 8 (Seq.length bs)));
     A.ghost_join (A.split_l a 8sz) (A.split_r a 8sz) adj;
     rewrite (A.pts_to (A.merge (A.split_l a 8sz) (A.split_r a 8sz)) _ _)
-            (A.pts_to a full_perm (spec_serialize_iv v));
-    intro_pure (seq_suffix_is_zero (spec_serialize_iv v) timestamp_len /\
-                spec_serialize_iv v == spec_serialize_iv v);
+            (A.pts_to a full_perm (spec_serializer_iv v));
+    intro_pure (seq_suffix_is_zero (spec_serializer_iv v) timestamp_len /\
+                spec_serializer_iv v == spec_serializer_iv v);
     return ()
+#pop-options
