steel/formats/README.md
@@ -1,0 +1,60 @@
+* qd/Zeta.Formats.Aux.rfc Contains the qd format of types used by Zeta
+
+  To rebuild, you need a build of EverParse
+    - `make quackyducky lowparse -jN` in everparse
+    - this should give you the qd executable and lowparse checked files
+
+  Set EVERPARSE_HOME to the working copy of EverParse
+  
+  Then, `make qd -jN` in this directory (steel/formats)
+  
+    - this will produce the parsers and serializers, both spec and
+      Low*, for the formats in the rfc
+
+    - Note, you can add OTHERFLAGS='--admit_smt_queries true' if
+      you're in a hurry and not building a final artifact
+    
+* To expose a parser and/or serializer for a type in the rfc
+
+  1. In $ZETA_HOME/steel/Zeta.Steel.LogEntry.Spec.fsti
+
+     Give the signatures for the parser and serializer spec
+
+  2. In $ZETA_HOME/steel/Zeta.Steel.LogEntry.fsti
+
+     Give the signature in Steel of the Low* implementation.
+     
+     The name needs to be prefixed with `zeta__` because the
+     declaration in the Steel interface has to match the name in the
+     Low* implementation and both are extracted with -no_prefix by
+     Karamel.
+
+     e.g., see zeta__serialize_stamped_record
+
+     We usually also include a wrapper without the zeta__ prefix, for
+     convenience of calling from Zeta.
+
+  3. Then, in the $ZETA_HOME/steel/formats/spec directory, edit
+     Zeta.Steel.LogEntry.Spec.fst, providing definitions for the
+     signatures assumed in the corresponding .fsti in step 1
+
+  4. Compile the spec directory using `make spec`
+
+  5. Then in $ZETA_HOME/steel/formats/lowstar/Zeta.LowStar.LogEntry.fsti
+
+     Add Low* signatures corresponding to the ones given in step 2
+     above. The parser and serializer types from Zeta.LowStar.Parser
+     are the Low* equivalent to the ones in Zeta.Steel.Parser
+
+  6. Then in $ZETA_HOME/steel/formats/lowstar/Zeta.LowStar.LogEntry.fst
+
+     Provide a Low* impl of the signatures given in 5 (using the
+     LowParse.Low combinators)
+
+  7. Then, do a `make` in $ZETA_HOME/steel/formats and that should
+     verify and extract everything
+  
+     
+
+
+  
